src/main/scala/fi/abo/it/actortool/merging/Utilities.scala
@@ -2,11 +2,11 @@ package fi.abo.it.actortool.merging
 
 import fi.abo.it.actortool._
 
-object ContractGuardToActorGuardTranslator extends ASTReplacingVisitor[Map[(String,Int), Id]] {
+object ContractGuardToActorGuardTranslator extends ASTReplacingVisitor[Map[(String,Int), Expr]] {
   
   val Sep = Constants.Sep
   
-  override def visitExpr(expr: Expr)(implicit map: Map[(String,Int), Id]): Expr = {
+  override def visitExpr(expr: Expr)(implicit map: Map[(String,Int), Expr]): Expr = {
     expr match {
       case IndexAccessor(Id(ch),SpecialMarker("@")) => map(ch,0)
       case fa@FunctionApp("int",arguments) => FunctionApp("int",arguments map visitExpr)
