src/main/scala/fi/abo/it/actortool/util/PriorityMapBuilder.scala
@@ -5,7 +5,7 @@ import fi.abo.it.actortool._
 object PriorityMapBuilder {
   
   def buildPriorityMap(actor: DFActor, subComponent: Boolean, alwaysUseContracts: Boolean): Map[AbstractAction,List[AbstractAction]] = {
-    if (subComponent && !actor.contractActions.isEmpty && (actor.isNetwork || alwaysUseContracts || actor.hasAnnotation("schedule")) ) {
+    if (subComponent && !actor.contractActions.isEmpty && (actor.isNetwork || alwaysUseContracts || actor.hasAnnotation("merge")) ) {
       return (actor.contractActions map { a => (a,Nil: List[AbstractAction]) }).toMap
     }
     
